BackTrans/Emulate.v
@@ -1,0 +1,39 @@
+Require Stlc.SpecSyntax.
+Require Utlc.SpecSyntax.
+Require Import BackTrans.UValHelpers.
+Require Import Stlc.SpecTyping.
+Require Import Stlc.StlcOmega.
+Require Import Stlc.LemmasTyping.
+Require Import Stlc.SpecEvaluation.
+Require Import Stlc.LemmasEvaluation.
+Require Import Utlc.SpecScoping.
+Require Import Utlc.LemmasScoping.
+Require Import Utlc.DecideEval.
+Require Import LogRel.PseudoType.
+Require Import LogRel.LemmasPseudoType.
+Require Import LogRel.LR.
+Require Import LogRel.LemmasLR.
+Require Import LogRel.LemmasIntro.
+Require Import Omega.
+Require Import Db.Lemmas.
+Require Import UVal.UVal.
+Require Utlc.Fix.
+
+Fixpoint emulate (n : nat) (t : U.UTm) : S.Tm :=
+  match t with
+    | U.wrong => stlcOmega (UVal n)
+    | U.var i => S.var i
+    | U.abs t => inArrDwn n (S.abs (UVal n) (emulate n t))
+    | U.app t₁ t₂ => S.unit
+    | U.unit => inUnitDwn n S.unit
+    | U.true => inBoolDwn n S.true
+    | U.false => inBoolDwn n S.false
+    | U.ite t₁ t₂ t₃ => S.unit
+    | U.pair t₁ t₂ => inProdDwn n (S.pair (emulate n t₁) (emulate n t₂))
+    | U.proj₁ t => S.unit
+    | U.proj₂ t => S.unit
+    | U.inl t => inSumDwn n (emulate n t)
+    | U.inr t => inSumDwn n (emulate n t)
+    | U.caseof t₁ t₂ t₃ => S.unit
+    | U.seq t₁ t₂ => S.unit
+  end.
