BackTrans/UValHelpers.v
@@ -1,0 +1,102 @@
+Require Import UVal.UVal.
+Require Import Utlc.LemmasScoping.
+Require Import Utlc.SpecSyntax.
+Require Import Stlc.SpecSyntax.
+Require Import Stlc.Inst.
+Require Import Stlc.SpecTyping.
+Require Import Stlc.SpecEvaluation.
+Require Import Stlc.LemmasTyping.
+Require Import Stlc.LemmasEvaluation.
+Require Import Stlc.CanForm.
+Require Import Db.Lemmas.
+Require Import Db.WellScoping.
+Require Import LogRel.LR.
+Require Import LogRel.LemmasLR.
+Require Import LogRel.LemmasIntro.
+Require Import LogRel.LemmasInversion.
+Require Import LogRel.LemmasPseudoType.
+Require Import LogRel.PseudoType.
+Require Import BackTrans.UpgradeDowngrade.
+Require Import Omega.
+
+
+Section Intro.
+  Definition inUnitDwn (n : nat) (t : Tm) := app (downgrade n 1) (inUnit n t).
+  Definition inBoolDwn (n : nat) (t : Tm) := app (downgrade n 1) (inBool n t).
+  Definition inProdDwn (n : nat) (t : Tm) := app (downgrade n 1) (inProd n t).
+  Definition inArrDwn (n : nat) (t : Tm) := app (downgrade n 1) (inArr n t).
+  Definition inSumDwn (n : nat) (t : Tm) := app (downgrade n 1) (inSum n t).
+End Intro.
+
+Section IntroProps.
+  Lemma termrel_inUnitDwn {d w n p vs vu} :
+    dir_world_prec n w d p →
+    valrel d w ptunit vs vu →
+    termrel d w (pEmulDV n p) (inUnitDwn n vs) vu.
+  Proof.
+   intros dwp vr. 
+   unfold inUnitDwn.
+   apply downgrade_works'; trivial.
+   replace (n + 1) with (S n) by omega.
+   apply valrel_inUnit'; trivial.
+  Qed.
+
+  Lemma termrel_inBoolDwn {d w n p vs vu} :
+    dir_world_prec n w d p →
+    valrel d w ptbool vs vu →
+    termrel d w (pEmulDV n p) (inBoolDwn n vs) vu.
+  Proof.
+   intros dwp vr. 
+   unfold inBoolDwn.
+   apply downgrade_works'; trivial.
+   replace (n + 1) with (S n) by omega.
+   apply valrel_inBool'; trivial.
+  Qed.
+
+  Lemma termrel_inProdDwn {d w n p vs vu} :
+    dir_world_prec n w d p →
+    valrel d w (ptprod (pEmulDV n p) (pEmulDV n p)) vs vu →
+    termrel d w (pEmulDV n p) (inProdDwn n vs) vu.
+  Proof.
+   intros dwp vr. 
+   unfold inProdDwn.
+   apply downgrade_works'; trivial.
+   replace (n + 1) with (S n) by omega.
+   apply valrel_inProd''; trivial.
+  Qed.
+
+  Lemma termrel_inSumDwn {d w n p vs vu} :
+    dir_world_prec n w d p →
+    valrel d w (ptsum (pEmulDV n p) (pEmulDV n p)) vs vu →
+    termrel d w (pEmulDV n p) (inSumDwn n vs) vu.
+  Proof.
+   intros dwp vr. 
+   unfold inProdDwn.
+   apply downgrade_works'; trivial.
+   replace (n + 1) with (S n) by omega.
+   apply valrel_inSum''; trivial.
+  Qed.
+
+  Lemma termrel_inArrDwn {d w n p vs vu} :
+    dir_world_prec n w d p →
+    valrel d w (ptarr (pEmulDV n p) (pEmulDV n p)) vs vu →
+    termrel d w (pEmulDV n p) (inArrDwn n vs) vu.
+  Proof.
+   intros dwp vr. 
+   unfold inArrDwn.
+   apply downgrade_works'; trivial.
+   replace (n + 1) with (S n) by omega.
+   apply valrel_inArr; trivial.
+  Qed.
+End IntroProps.
+
+Section Destruct.
+  Definition caseUnitDwn (n : nat) (t : Tm) := app (downgrade n 1) (inUnit n t).
+  Definition inBoolDwn (n : nat) (t : Tm) := app (downgrade n 1) (inBool n t).
+  Definition inProdDwn (n : nat) (t : Tm) := app (downgrade n 1) (inProd n t).
+  Definition inArrDwn (n : nat) (t : Tm) := app (downgrade n 1) (inArr n t).
+  Definition inSumDwn (n : nat) (t : Tm) := app (downgrade n 1) (inSum n t).
+End Destruct.
+
+Section DestructProps.
+End DestructProps.
